theories/theories/utp_csp.thy
@@ -1,0 +1,18 @@
+(******************************************************************************)
+(* Project: Mechanisation of the UTP                                          *)
+(* File: utp_csp.thy                                                          *)
+(* Authors: Samuel Canham and Simon Foster, University of York                *)
+(******************************************************************************)
+
+header {* CSP Processes *}
+
+theory utp_csp
+imports 
+  utp_designs
+  utp_theory
+  utp_reactive
+begin
+
+
+
+end
